Refactor : use pow

src/part1.lean
@@ -5,92 +5,73 @@ namespace linear_map
 
 variables {E K : Type*} [field K] [add_comm_group E] [vector_space K E] (f : E →ₗ[K] E)
 
-def iterate (n : ℕ) : E →ₗ[K] E :=
-{ to_fun := λ x, f^[n] x,
-  map_add' := 
-  begin
-    induction n with n hn,
-    { simp },
-    { simp [hn] }
-  end,
-  map_smul' := 
-  begin
-    induction n with n hn,
-    { simp },
-    { simp [hn] }
-  end }
--- try to simplify by grouping proofs
+lemma pow_succ_apply (n : ℕ) (x : E) : (f^(n+1)) x = f ((f^n) x) :=
+by rw [pow_succ]; refl
 
-lemma iterate_succ_apply (n : ℕ) (x : E) : f.iterate (n+1) x = (f.iterate n (f x)) :=
-  function.iterate_succ_apply f n x
+lemma pow_succ_apply' (n : ℕ) (x : E) : (f^(n+1)) x = (f^n) (f x) :=
+by rw [pow_succ']; refl
 
-lemma iterate_succ_apply' (n : ℕ) (x : E) : f.iterate (n+1) x = f (f.iterate n x) :=
-  function.iterate_succ_apply' f n x
+lemma pow_add_apply (n m : ℕ) (x : E) : (f^(n+m)) x = (f^n) ((f^m) x) :=
+by rw [pow_add]; refl
 
-lemma iterate_add_apply (m n : ℕ) (x : E) : f.iterate (m+n) x = f.iterate m (f.iterate n x) :=
-  function.iterate_add_apply f m n x
-
-lemma iterate_add_apply' (m n : ℕ) (x : E) : f.iterate (m+n) x = f.iterate n (f.iterate m x) :=
-  add_comm n m ▸ function.iterate_add_apply f n m x
-
-lemma iterate_succ (n : ℕ) : f.iterate (n+1) = (f.iterate n).comp f :=
-  ext (f.iterate_succ_apply n)
-
-lemma iterate_succ' (n : ℕ) : f.iterate (n+1) = f.comp (f.iterate n) :=
-  ext (f.iterate_succ_apply' n)
-
-lemma iterate_stable {U : submodule K E} (hU : ∀ x ∈ U, f x ∈ U) :
-  ∀ n, ∀ x ∈ U, f.iterate n x ∈ U
-| 0 := λ x hx, hx
-| (n+1) := λ x hx, (iterate_stable n _ (hU x hx))
+lemma pow_add_apply' (n m : ℕ) (x : E) : (f^(n+m)) x = (f^m) ((f^n) x) :=
+by rw [add_comm]; exact f.pow_add_apply m n x
 
 lemma comp_stable (g : E →ₗ[K] E) {U : submodule K E} (hfU : ∀ x ∈ U, f x ∈ U)
   (hgU : ∀ x ∈ U, g x ∈ U) : ∀ x ∈ U, (f.comp g) x ∈ U := 
 λ x hx, hfU _ (hgU x hx)
+
+lemma pow_stable {U : submodule K E} (hfU : ∀ x ∈ U, f x ∈ U) :
+  ∀ (n : ℕ), ∀ x ∈ U, (f^n) x ∈ U
+| 0 := λ x hx, hx
+| (n+1) := λ x hx,
+  begin
+    rw pow_succ_apply,
+    exact hfU _ (pow_stable n _ hx)
+  end
 
 lemma restrict_comp (g : E →ₗ[K] E) {U : submodule K E} (hfU : ∀ x ∈ U, f x ∈ U)
   (hgU : ∀ x ∈ U, g x ∈ U) (hfgU : ∀ x ∈ U, (f.comp g) x ∈ U) : 
   (f.comp g).restrict hfgU = (f.restrict hfU).comp (g.restrict hgU) :=
 rfl
 
-lemma iterate_restrict_comm {U : submodule K E} (hU : ∀ x ∈ U, f x ∈ U) :
-  ∀ n, (f.restrict hU).iterate n = (f.iterate n).restrict (f.iterate_stable hU n)
+lemma pow_restrict_comm {U : submodule K E} (hfU : ∀ x ∈ U, f x ∈ U) :
+  ∀ n, (f.restrict hfU)^n = (f^n).restrict (f.pow_stable hfU n)
 | 0 := 
   begin
     ext ⟨x, hx⟩,
-    simp [iterate, function.iterate_zero],
     refl
   end
 | (n+1) :=
   begin
     ext ⟨x, hx⟩,
-    simp [iterate_succ', restrict_comp _ _ hU (f.iterate_stable hU n) _],
-    rw iterate_restrict_comm n
+    simp only [pow_succ, mul_eq_comp, restrict_comp _ _ hfU (f.pow_stable hfU n) _],
+    rw pow_restrict_comm n
   end
 
-def ker_it (n : ℕ) := (f.iterate n).ker
+def ker_it (n : ℕ) := (f^n).ker
 
 lemma mem_ker_it_succ_iff (n : ℕ) (x : E) : x ∈ f.ker_it (n+1) ↔ f x ∈ f.ker_it n :=
-by rw [ker_it, mem_ker, ker_it, mem_ker, iterate_succ_apply]
+by rw [ker_it, mem_ker, ker_it, mem_ker, pow_succ']; refl
 
-def range_it (n : ℕ) := (f.iterate n).range
+def range_it (n : ℕ) := (f^n).range
 
 lemma range_it_succ_eq' (n : ℕ) : f.range_it (n+1) = (f.range_it n).map f :=
-by rw [range_it, range_it, range, range, iterate_succ', submodule.map_comp]
+by rw [range_it, range_it, range, range, pow_succ, mul_eq_comp, submodule.map_comp]
 
-lemma range_it_succ_eq (n : ℕ) : f.range_it (n+1) = f.range.map (f.iterate n) :=
-by rw [range_it, range, range, iterate_succ, submodule.map_comp]
+lemma range_it_succ_eq (n : ℕ) : f.range_it (n+1) = f.range.map (f^n) :=
+by rw [range_it, range, range, pow_succ', mul_eq_comp, submodule.map_comp]
 
 lemma ker_it_mono : monotone f.ker_it :=
 monotone_of_monotone_nat
 begin
   intros n x hx,
   rw [ker_it, mem_ker] at ⊢ hx,
-  simp [hx, iterate_succ_apply']
+  simp [hx, pow_succ]
 end
 
 lemma range_it_antimono : ∀ ⦃x y⦄, x ≤ y → f.range_it y ≤ f.range_it x :=
-antimono_of_antimono_nat (λ n x ⟨x', _, hx'⟩, ⟨f x', trivial, hx'⟩)
+antimono_of_antimono_nat (λ n x ⟨x', _, hx'⟩, ⟨f x', trivial, by simpa using hx'⟩)
 
 lemma q1_1 {m : ℕ} (hm : f.range_it (m+1) = f.range_it m) : ∀ p, f.range_it (m+p) = f.range_it m
 | 0 := rfl
